Updated examples

lean4/Automaton/Regex/Char.lean
@@ -15,10 +15,10 @@ def char_δ (a : σs) : char_qs → σs → Finset char_qs
   | ⟨1, _⟩ , s => if s = a then {⟨2, by simp⟩} else {}
   | _ , _ => {}
 
-def char (a : σs) : NFA σs := {qs := char_qs, q₀ := {⟨1,by simp⟩}, fs := {⟨2,by simp⟩}, δ := char_δ a }
+def char_nfa (a : σs) : NFA σs := {qs := char_qs, q₀ := {⟨1,by simp⟩}, fs := {⟨2,by simp⟩}, δ := char_δ a }
 
-theorem accepts_iff (a : σs) : nfa_accepts (char a) w ↔ w = [a] := by
-  simp only [nfa_accepts,char]
+theorem accepts_iff (a : σs) : nfa_accepts (char_nfa a) w ↔ w = [a] := by
+  simp only [nfa_accepts,char_nfa]
   apply Iff.intro
   · intro ne
     rw [Finset.Nonempty] at ne
