lean4/Automaton/NFA/ENFA.lean
@@ -64,7 +64,7 @@ lemma εclosure_eq_εclosure : εclosure tn f = if h : f = (f.biUnion (fun q => 
 theorem εclosure_empty_empty : εclosure tn ∅ = ∅ := by
   rw [εclosure_eq_εclosure]
   simp
-  
+
 
 lemma εclosure_start_mem (q : tn.qs) (f : Finset tn.qs) : q ∈ f → q ∈ εclosure tn f := by
   rw [εclosure_eq_εclosure]
@@ -201,8 +201,6 @@ theorem εnfa_to_dfa_eq : εnfa_accepts tn w ↔ dfa_accepts (εnfa_to_dfa tn) w
     have := ToDFA.nfa_to_dfa_eq (εnfa_to_nfa tn) w
     apply this.mpr
     exact e
-
-
 
 
 end εNFA
